Weidenbach_Book/DPLL_NOT.thy
@@ -1,0 +1,278 @@
+theory DPLL_NOT
+imports CDCL_NOT
+begin
+
+section \<open>DPLL as an instance of NOT\<close>
+subsection \<open>DPLL with simple backtrack\<close>
+locale dpll_with_backtrack
+begin
+inductive backtrack :: "('v, dpll_marked_level, dpll_mark) marked_lit list \<times> 'v clauses
+  \<Rightarrow> ('v, dpll_marked_level, dpll_mark) marked_lit list \<times> 'v clauses \<Rightarrow> bool" where
+"backtrack_split (fst S)  = (M', L # M) \<Longrightarrow> is_marked L \<Longrightarrow> D \<in># snd S
+  \<Longrightarrow> fst S \<Turnstile>as CNot D \<Longrightarrow> backtrack S (Propagated (- (lit_of L)) Proped # M, snd S)"
+
+inductive_cases backtrackE[elim]: "backtrack (M, N) (M', N')"
+lemma backtrack_is_backjump:
+  fixes M M' :: "('v, dpll_marked_level, dpll_mark) marked_lit list"
+  assumes
+    backtrack: "backtrack (M, N) (M', N')" and
+    no_dup: "(no_dup \<circ> fst) (M, N)" and
+    decomp: "all_decomposition_implies_m N (get_all_marked_decomposition M)"
+    shows "
+       \<exists>C F' K d F L l C'.
+          M = F' @ Marked K d # F \<and>
+          M' = Propagated L l # F \<and> N = N' \<and> C \<in># N \<and> F' @ Marked K d # F \<Turnstile>as CNot C \<and>
+          undefined_lit L F \<and> atm_of L \<in> atms_of_mu N \<union> atm_of ` lits_of (F' @ Marked K d # F) \<and>
+          N \<Turnstile>pm C' + {#L#} \<and> F \<Turnstile>as CNot C'"
+proof -
+  let ?S = "(M, N)"
+  let ?T = "(M', N')"
+  obtain F F' P L D where
+    b_sp: "backtrack_split M = (F', L # F)"  and
+    "is_marked L" and
+    "D \<in># snd ?S" and
+    "M \<Turnstile>as CNot D" and
+    bt: "backtrack ?S (Propagated (- (lit_of L)) P # F, N)" and
+    M': "M' = Propagated (- (lit_of L)) P # F" and
+    [simp]: "N' = N"
+  using backtrackE[OF backtrack] by (metis backtrack fstI sndI)
+  let ?K = "lit_of L"
+  let ?C = "image_mset lit_of {#K\<in>#mset M. is_marked K \<and> K\<noteq>L#} :: 'v literal multiset"
+  let ?C' = "set_mset (image_mset single (?C+{#?K#}))"
+  obtain K d where L: "L = Marked K d" using \<open>is_marked L\<close> by (cases L) auto
+
+  have M: "M = F' @ Marked K d # F"
+    using b_sp  by (metis L backtrack_split_list_eq fst_conv snd_conv)
+  moreover have "F' @ Marked K d # F \<Turnstile>as CNot D"
+    using \<open>M\<Turnstile>as CNot D\<close> unfolding M .
+  moreover have "undefined_lit (-?K) F"
+    using no_dup unfolding M L by (simp add: defined_lit_map)
+  moreover have "atm_of (-K) \<in> atms_of_mu N \<union> atm_of ` lits_of (F' @ Marked K d # F)"
+    by auto
+  moreover
+    have "set_mset N \<union> ?C' \<Turnstile>ps {{#}}"
+      proof -
+        have A: "set_mset N \<union> ?C' \<union> (\<lambda>a. {#lit_of a#}) ` set M  =
+          set_mset  N \<union> (\<lambda>a. {#lit_of a#}) ` set M"
+          unfolding M L by auto
+        have "set_mset  N \<union> {{#lit_of L#} |L. is_marked L \<and> L \<in> set M}
+            \<Turnstile>ps (\<lambda>a. {#lit_of a#}) ` set M"
+          using all_decomposition_implies_propagated_lits_are_implied[OF decomp] .
+        moreover have C': "?C' = {{#lit_of L#} |L. is_marked L \<and> L \<in> set M}"
+          unfolding M L apply standard
+            apply force
+          using IntI by auto
+        ultimately have N_C_M: "set_mset N \<union> ?C' \<Turnstile>ps (\<lambda>a. {#lit_of a#}) ` set M"
+          by auto
+        have "set_mset N \<union> (\<lambda>L. {#lit_of L#}) ` (set M) \<Turnstile>ps {{#}}"
+          unfolding true_clss_clss_def
+          proof (intro allI impI, goal_cases)
+            case (1 I) note tot = this(1) and cons = this(2) and I_N_M = this(3)
+            have "I \<Turnstile> D"
+              using I_N_M \<open>D \<in># snd ?S\<close> unfolding true_clss_def by auto
+            moreover have "I \<Turnstile>s CNot D"
+              using \<open>M \<Turnstile>as CNot D\<close> unfolding M by (metis "1"(3) \<open>M \<Turnstile>as CNot D\<close>
+                true_annots_true_cls true_cls_mono_set_mset_l true_clss_def
+                true_clss_singleton_lit_of_implies_incl true_clss_union)
+            ultimately show ?case using cons consistent_CNot_not by blast
+          qed
+        thus ?thesis
+          using true_clss_clss_left_right[OF N_C_M, of "{{#}}"] unfolding A by auto
+      qed
+    have "N \<Turnstile>pm image_mset uminus ?C + {#-?K#}"
+      unfolding true_clss_cls_def true_clss_clss_def total_over_m_def
+      proof (intro allI impI)
+        fix I
+        assume
+          tot: "total_over_set I (atms_of_m (set_mset N \<union> {image_mset uminus ?C + {#- ?K#}})) " and
+          cons: "consistent_interp I" and
+          "I \<Turnstile>sm N"
+        have "(K \<in> I \<and> -K \<notin> I) \<or> (-K \<in> I \<and> K \<notin> I)"
+          using cons tot unfolding consistent_interp_def L by (cases K) auto
+        have "total_over_set I (atm_of ` lit_of ` (set M \<inter> {L. is_marked L \<and> L \<noteq> Marked K d}))"
+          using tot by (auto simp add: L atms_of_uminus_lit_atm_of_lit_of)
+
+        hence H: "\<And>x.
+            lit_of x \<notin> I \<Longrightarrow> x \<in> set M \<Longrightarrow>is_marked x
+            \<Longrightarrow> x \<noteq> Marked K d \<Longrightarrow> -lit_of x \<in> I"
+            (* TODO one-liner? *)
+          unfolding total_over_set_def atms_of_s_def
+          proof -
+            fix x :: "('v, dpll_marked_level, dpll_mark) marked_lit"
+            assume a1: "x \<in> set M"
+            assume a2: "\<forall>l\<in>atm_of ` lit_of ` (set M \<inter> {L. is_marked L \<and> L \<noteq> Marked K d}).
+              Pos l \<in> I \<or> Neg l \<in> I"
+            assume a3: "lit_of x \<notin> I"
+            assume a4: "is_marked x"
+            assume a5: "x \<noteq> Marked K d"
+            have f6: "Neg (atm_of (lit_of x)) = - Pos (atm_of (lit_of x))"
+              by simp
+            have "Pos (atm_of (lit_of x)) \<in> I \<or> Neg (atm_of (lit_of x)) \<in> I"
+              using a5 a4 a2 a1 by blast
+            thus "- lit_of x \<in> I"
+              using f6 a3 by (metis (no_types) atm_of_in_atm_of_set_iff_in_set_or_uminus_in_set
+                literal.sel(1))
+          qed
+        have "\<not>I \<Turnstile>s ?C'"
+          using \<open>set_mset N \<union> ?C' \<Turnstile>ps {{#}}\<close> tot cons \<open>I \<Turnstile>sm N\<close>
+          unfolding true_clss_clss_def total_over_m_def
+          by (simp add: atms_of_uminus_lit_atm_of_lit_of atms_of_m_single_image_atm_of_lit_of)
+        then show "I \<Turnstile> image_mset uminus ?C + {#- lit_of L#}"
+          unfolding true_clss_def true_cls_def Bex_mset_def
+          using \<open>(K \<in> I \<and> -K \<notin> I) \<or> (-K \<in> I \<and> K \<notin> I)\<close>
+          unfolding L by (auto dest!: H)
+      qed
+  moreover
+    have "set F' \<inter> {K. is_marked K \<and> K \<noteq> L} = {}"
+      using backtrack_split_fst_not_marked[of _ M] b_sp by auto
+    hence "F \<Turnstile>as CNot (image_mset uminus ?C)"
+       unfolding M CNot_def true_annots_def by (auto simp add: L lits_of_def)
+  ultimately show ?thesis
+    using M' \<open>D \<in># snd ?S\<close> L by auto
+qed
+
+lemma backtrack_is_backjump':
+  fixes M M' :: "('v, dpll_marked_level, dpll_mark) marked_lit list"
+  assumes
+    backtrack: "backtrack S T" and
+    no_dup: "(no_dup \<circ> fst) S" and
+    decomp: "all_decomposition_implies_m (snd S) (get_all_marked_decomposition (fst S))"
+    shows "
+        \<exists>C F' K d F L l C'.
+          fst S = F' @ Marked K d # F \<and>
+          T = (Propagated L l # F, snd S) \<and> C \<in># snd S \<and> fst S \<Turnstile>as CNot C
+          \<and> undefined_lit L F \<and> atm_of L \<in> atms_of_mu (snd S) \<union> atm_of ` lits_of (fst S) \<and>
+          snd S \<Turnstile>pm C' + {#L#} \<and> F \<Turnstile>as CNot C'"
+  apply (cases S, cases T)
+  using backtrack_is_backjump[of "fst S" "snd S" "fst T" "snd T"] assms by fastforce
+
+sublocale dpll_state fst snd "\<lambda>L (M, N). (L # M, N)" "\<lambda>(M, N). (tl M, N)"
+  "\<lambda>C (M, N). (M, {#C#} + N)" "\<lambda>C (M, N). (M, remove_mset N C)"
+  by unfold_locales auto
+
+sublocale backjumping_ops fst snd "\<lambda>L (M, N). (L # M, N)" "\<lambda>(M, N). (tl M, N)"
+  "\<lambda>C (M, N). (M, {#C#} + N)" "\<lambda>C (M, N). (M, remove_mset N C)" "\<lambda>_ _ S T. backtrack S T"
+  by unfold_locales
+
+lemma backtrack_is_backjump'':
+  fixes M M' :: "('v, dpll_marked_level, dpll_mark) marked_lit list"
+  assumes
+    backtrack: "backtrack S T" and
+    no_dup: "(no_dup \<circ> fst) S" and
+    decomp: "all_decomposition_implies_m (snd S) (get_all_marked_decomposition (fst S))"
+    shows "backjump S T"
+proof -
+  obtain C F' K d F L l C' where
+    1: "fst S = F' @ Marked K d # F" and
+    2: "T = (Propagated L l # F, snd S)" and
+    3: "C \<in># snd S" and
+    4: "fst S \<Turnstile>as CNot C" and
+    5: "undefined_lit L F" and
+    6: "atm_of L \<in> atms_of_mu (snd S) \<union> atm_of ` lits_of (fst S)" and
+    7: "snd S \<Turnstile>pm C' + {#L#}" and
+    8: "F \<Turnstile>as CNot C'"
+  using backtrack_is_backjump'[OF assms] by blast
+  show ?thesis
+    using backjump.intros[OF 1 _ 3 4 5 6 7 8] 2 backtrack 1
+    by (auto simp: state_eq\<^sub>N\<^sub>O\<^sub>T_def simp del: state_simp\<^sub>N\<^sub>O\<^sub>T)
+qed
+
+lemma can_do_bt_step:
+   assumes
+     M: "fst S = F' @ Marked K d # F" and
+     "C \<in># snd S" and
+     C: "fst S \<Turnstile>as CNot C"
+   shows "\<not> no_step backtrack S"
+proof -
+  obtain L G' G where
+    "backtrack_split (fst S) = (G', L # G)"
+    unfolding M by (induction F' rule: marked_lit_list_induct) auto
+  moreover hence "is_marked L"
+     by (metis backtrack_split_snd_hd_marked list.distinct(1) list.sel(1) snd_conv)
+  ultimately show ?thesis
+     using backtrack.intros[of S G' L G C] \<open>C \<in># snd S\<close> C unfolding M by auto
+qed
+
+end
+
+sublocale dpll_with_backtrack \<subseteq> dpll_with_backjumping_ops fst snd "\<lambda>L (M, N). (L # M, N)"
+  "\<lambda>(M, N). (tl M, N)" "\<lambda>C (M, N). (M, {#C#} + N)" "\<lambda>C (M, N). (M, remove_mset N C)" "\<lambda>_. True"
+  "\<lambda>(M, N). no_dup M \<and> all_decomposition_implies_m N (get_all_marked_decomposition M)"
+  "(\<lambda>_ _ S T. backtrack S T)"
+  by unfold_locales (metis (mono_tags, lifting) dpll_with_backtrack.backtrack_is_backjump''
+   dpll_with_backtrack.can_do_bt_step prod.case_eq_if comp_apply)
+
+sublocale dpll_with_backtrack \<subseteq> dpll_with_backjumping fst snd "\<lambda>L (M, N). (L # M, N)"
+  "\<lambda>(M, N). (tl M, N)" "\<lambda>C (M, N). (M, {#C#} + N)" "\<lambda>C (M, N). (M, remove_mset N C)" "\<lambda>_. True"
+  "\<lambda>(M, N). no_dup M \<and> all_decomposition_implies_m N (get_all_marked_decomposition M)"
+  "(\<lambda>_ _ S T. backtrack S T)"
+  apply unfold_locales
+  using dpll_bj_no_dup dpll_bj_all_decomposition_implies_inv apply fastforce
+  done
+
+sublocale dpll_with_backtrack \<subseteq> conflict_driven_clause_learning_ops
+  fst snd "\<lambda>L (M, N). (L # M, N)"
+  "\<lambda>(M, N). (tl M, N)" "\<lambda>C (M, N). (M, {#C#} + N)" "\<lambda>C (M, N). (M, remove_mset N C)" "\<lambda>_. True"
+  "\<lambda>(M, N). no_dup M \<and> all_decomposition_implies_m N (get_all_marked_decomposition M)"
+  "(\<lambda>_ _ S T. backtrack S T)" "\<lambda>_ _. False" "\<lambda>_ _. False"
+  by unfold_locales
+
+sublocale dpll_with_backtrack \<subseteq> conflict_driven_clause_learning
+  fst snd "\<lambda>L (M, N). (L # M, N)"
+  "\<lambda>(M, N). (tl M, N)" "\<lambda>C (M, N). (M, {#C#} + N)" "\<lambda>C (M, N). (M, remove_mset N C)" "\<lambda>_. True"
+  "\<lambda>(M, N). no_dup M \<and> all_decomposition_implies_m N (get_all_marked_decomposition M)"
+  "(\<lambda>_ _ S T. backtrack S T)" "\<lambda>_ _. False" "\<lambda>_ _. False"
+  apply unfold_locales
+  using cdcl\<^sub>N\<^sub>O\<^sub>T.simps dpll_bj_inv forgetE learnE by blast
+
+context dpll_with_backtrack
+begin
+lemma tranclp_dpll_wf_inital_state:
+  assumes fin: "finite A"
+  shows "wf {((M'::('v, dpll_marked_level, dpll_mark) marked_lits, N'::'v clauses), ([], N))|M' N' N.
+    dpll_bj\<^sup>+\<^sup>+ ([], N) (M', N') \<and> atms_of_mu N \<subseteq> atms_of_m A}"
+  using tranclp_dpll_bj_wf[OF assms(1)] by (rule wf_subset) auto
+
+theorem full0_dpll_normal_forms:
+  fixes M M' :: "('v, dpll_marked_level, dpll_mark) marked_lit list"
+  assumes
+    full: "full0 dpll_bj ([], N) (M', N')"
+  shows "unsatisfiable (set_mset N) \<or> (M' \<Turnstile>asm N \<and> satisfiable (set_mset N))"
+  using assms full0_dpll_backjump_normal_forms[of "([],N)" "(M', N')" "set_mset N"] by auto
+
+lemma cdcl\<^sub>N\<^sub>O\<^sub>T_is_dpll:
+  "cdcl\<^sub>N\<^sub>O\<^sub>T S T \<longleftrightarrow> dpll_bj S T"
+  by (auto simp: cdcl\<^sub>N\<^sub>O\<^sub>T.simps learn.simps forget\<^sub>N\<^sub>O\<^sub>T.simps)
+
+text \<open>Another proof of termination:\<close>
+lemma "wf {(T, S). dpll_bj S T \<and> cdcl\<^sub>N\<^sub>O\<^sub>T_NOT_all_inv A S}"
+  unfolding cdcl\<^sub>N\<^sub>O\<^sub>T_is_dpll[symmetric]
+  by (rule wf_cdcl\<^sub>N\<^sub>O\<^sub>T_no_learn_and_forget_infinite_chain)
+  (auto simp: learn.simps forget\<^sub>N\<^sub>O\<^sub>T.simps)
+end
+
+subsection \<open>Adding restarts\<close>
+locale dpll_withbacktrack_and_restarts =
+  dpll_with_backtrack +
+  fixes f :: "nat \<Rightarrow> nat"
+  assumes strict_mono: "strict_mono f"
+begin
+  sublocale cdcl\<^sub>N\<^sub>O\<^sub>T_increasing_restarts  fst snd "\<lambda>L (M, N). (L # M, N)" "\<lambda>(M, N). (tl M, N)"
+    "\<lambda>C (M, N). (M, {#C#} + N)" "\<lambda>C (M, N). (M, remove_mset N C)" f "\<lambda>(_, N) S. S = ([], N)"
+  "\<lambda>A (M, N). atms_of_mu N \<subseteq> atms_of_m A \<and> atm_of ` lits_of M \<subseteq> atms_of_m A \<and> finite A
+    \<and> all_decomposition_implies_m N (get_all_marked_decomposition M)"
+  "\<lambda>A T. (2+card (atms_of_m A)) ^ (1+card (atms_of_m A))
+               - \<mu>\<^sub>C (1+card (atms_of_m A)) (2+card (atms_of_m A)) (trail_weight T)" dpll_bj
+  "\<lambda>(M, N). no_dup M \<and> all_decomposition_implies_m N (get_all_marked_decomposition M)"
+  "\<lambda>A _.  (2+card (atms_of_m A)) ^ (1+card (atms_of_m A))"
+  apply unfold_locales
+         apply (rule strict_mono)
+        apply (smt dpll_bj_all_decomposition_implies_inv dpll_bj_atms_in_trail_in_set
+          dpll_bj_clauses dpll_bj_no_dup prod.case_eq_if)
+       apply (rule dpll_bj_trail_mes_decreasing_prop; auto)
+      apply (case_tac T, simp)
+     apply (case_tac U, simp)
+    using dpll_bj_clauses dpll_bj_all_decomposition_implies_inv dpll_bj_no_dup by fastforce+
+end
+
+end
